src/opt/SimPromises.v
@@ -175,21 +175,21 @@ Module SimPromises.
     econs. ii. eapply H; eauto.
   Qed.
 
-  Definition none_if loc ts (none_for:t) (released:option View.t): option View.t :=
-    if mem loc ts none_for
+  Definition none_if loc ts (pview:t) (released:option View.t): option View.t :=
+    if mem loc ts pview
     then None
     else released.
 
-  Definition mem_le_transf (none_for:t) (lhs rhs:Memory.t): Prop :=
+  Definition mem_le_transf (pview:t) (lhs rhs:Memory.t): Prop :=
     forall loc to from val released
       (LHS: Memory.get loc to lhs = Some (from, Message.mk val released)),
-      Memory.get loc to rhs = Some (from, Message.mk val (none_if loc to none_for released)).
+      Memory.get loc to rhs = Some (from, Message.mk val (none_if loc to pview released)).
 
-  Definition kind_transf loc ts (none_for:t) (kind:Memory.op_kind): Memory.op_kind :=
+  Definition kind_transf loc ts (pview:t) (kind:Memory.op_kind): Memory.op_kind :=
     match kind with
     | Memory.op_kind_add => Memory.op_kind_add
-    | Memory.op_kind_split ts val rel => Memory.op_kind_split ts val (none_if loc ts none_for rel)
-    | Memory.op_kind_lower rel => Memory.op_kind_lower (none_if loc ts none_for rel)
+    | Memory.op_kind_split ts val rel => Memory.op_kind_split ts val (none_if loc ts pview rel)
+    | Memory.op_kind_lower rel => Memory.op_kind_lower (none_if loc ts pview rel)
     end.
 
   Lemma kind_transf_bot loc ts kind:
@@ -198,10 +198,10 @@ Module SimPromises.
     destruct kind; ss.
   Qed.
 
-  Inductive sem (none_for:t) (inv:t) (promises_src promises_tgt:Memory.t): Prop :=
+  Inductive sem (pview:t) (inv:t) (promises_src promises_tgt:Memory.t): Prop :=
   | sem_intro
-      (LE: mem_le_transf none_for promises_tgt promises_src)
-      (NONEFOR: forall l t (MEM: mem l t none_for), exists f msg, Memory.get l t promises_tgt = Some (f, msg))
+      (LE: mem_le_transf pview promises_tgt promises_src)
+      (PVIEW: forall l t (MEM: mem l t pview), exists f msg, Memory.get l t promises_tgt = Some (f, msg))
       (SOUND: forall l t (INV: mem l t inv),
           Memory.get l t promises_tgt = None /\
           exists f v r, Memory.get l t promises_src = Some (f, Message.mk v r))
@@ -212,19 +212,19 @@ Module SimPromises.
   .
 
   Lemma promise
-        none_for inv
+        pview inv
         loc from to val released
         promises1_src mem1_src
         promises1_tgt mem1_tgt promises2_tgt mem2_tgt
         kind_tgt
         (PROMISE_TGT: Memory.promise promises1_tgt mem1_tgt loc from to val released promises2_tgt mem2_tgt kind_tgt)
-        (INV1: sem none_for inv promises1_src promises1_tgt)
+        (INV1: sem pview inv promises1_src promises1_tgt)
         (SIM1: sim_memory mem1_src mem1_tgt)
         (LE1_SRC: Memory.le promises1_src mem1_src)
         (LE1_TGT: Memory.le promises1_tgt mem1_tgt):
     exists promises2_src mem2_src,
-      <<PROMISE_SRC: Memory.promise promises1_src mem1_src loc from to val (none_if loc to none_for released) promises2_src mem2_src (kind_transf loc to none_for kind_tgt)>> /\
-      <<INV2: sem none_for inv promises2_src promises2_tgt>> /\
+      <<PROMISE_SRC: Memory.promise promises1_src mem1_src loc from to val (none_if loc to pview released) promises2_src mem2_src (kind_transf loc to pview kind_tgt)>> /\
+      <<INV2: sem pview inv promises2_src promises2_tgt>> /\
       <<SIM2: sim_memory mem2_src mem2_tgt>>.
   Proof.
     inv PROMISE_TGT.
@@ -239,7 +239,7 @@ Module SimPromises.
       exploit sim_memory_add; try apply SIM1; try refl; eauto. i.
       esplits; eauto.
       + unfold none_if. condtac.
-        { inv INV1. exploit NONEFOR; eauto. i. des.
+        { inv INV1. exploit PVIEW; eauto. i. des.
           hexploit Memory.add_get0; try exact PROMISES; eauto. congr.
         }
         econs 1; eauto.
@@ -248,11 +248,11 @@ Module SimPromises.
           erewrite (@Memory.add_o promises2_tgt) in LHS; try exact PROMISES. revert LHS.
           condtac; ss.
           { i. des. inv LHS. unfold none_if. condtac; ss.
-            inv INV1. exploit NONEFOR; eauto. i. des.
+            inv INV1. exploit PVIEW; eauto. i. des.
             exploit Memory.add_get0; try exact PROMISES; eauto. congr.
           }
           { apply INV1. }
-        * i. inv INV1. exploit NONEFOR; eauto. i. des.
+        * i. inv INV1. exploit PVIEW; eauto. i. des.
           erewrite Memory.add_o; eauto. condtac; eauto.
         * i. inv INV1. exploit SOUND; eauto. i.
           erewrite Memory.add_o; eauto. erewrite (@Memory.add_o promises2); eauto.
@@ -270,7 +270,7 @@ Module SimPromises.
       exploit sim_memory_split; try apply SIM1; try refl; eauto. i.
       esplits; eauto.
       + unfold none_if. condtac.
-        { inv INV1. exploit NONEFOR; eauto. i. des.
+        { inv INV1. exploit PVIEW; eauto. i. des.
           hexploit Memory.split_get0; try exact PROMISES; eauto. congr.
         }
         econs 2; eauto.
@@ -279,12 +279,12 @@ Module SimPromises.
           erewrite Memory.split_o; eauto. erewrite (@Memory.split_o mem2); try exact x0.
           repeat condtac; ss.
           { i. des. inv LHS. unfold none_if. condtac; ss.
-            inv INV1. exploit NONEFOR; eauto. i. des.
+            inv INV1. exploit PVIEW; eauto. i. des.
             exploit Memory.split_get0; try exact PROMISES; eauto. congr.
           }
           { guardH o. i. des. inv LHS. ss. }
           { apply INV1. }
-        * i. inv INV1. exploit NONEFOR; eauto. i. des.
+        * i. inv INV1. exploit PVIEW; eauto. i. des.
           erewrite Memory.split_o; eauto. repeat condtac; eauto.
         * i. inv INV1. exploit SOUND; eauto. i.
           erewrite Memory.split_o; eauto. erewrite (@Memory.split_o mem2); eauto.
@@ -297,7 +297,7 @@ Module SimPromises.
           erewrite Memory.split_o; eauto. erewrite (@Memory.split_o promises2_tgt); eauto.
           repeat condtac; ss. inv INV1. eapply COMPLETE; eauto.
     - exploit Memory.lower_get0; try exact PROMISES; eauto. i.
-      exploit (@Memory.lower_exists promises1_src loc from to val (none_if loc to none_for released0) (none_if loc to none_for released));
+      exploit (@Memory.lower_exists promises1_src loc from to val (none_if loc to pview released0) (none_if loc to pview released));
         try by inv MEM; inv LOWER.
       { apply INV1. eauto. }
       { unfold none_if. condtac; ss.
@@ -319,7 +319,7 @@ Module SimPromises.
           condtac; ss.
           { i. des. inv LHS. ss. }
           { apply INV1. }
-        * i. inv INV1. exploit NONEFOR; eauto. i. des.
+        * i. inv INV1. exploit PVIEW; eauto. i. des.
           erewrite Memory.lower_o; eauto. condtac; eauto.
         * i. inv INV1. exploit SOUND; eauto. i.
           erewrite Memory.lower_o; eauto. erewrite (@Memory.lower_o mem2); eauto.
@@ -355,17 +355,17 @@ Module SimPromises.
   Qed.
 
   Lemma remove_tgt
-        none_for inv
+        pview inv
         loc from to val released
         promises1_src mem1_src
         promises1_tgt mem1_tgt promises2_tgt
         (REMOVE_TGT: Memory.remove promises1_tgt loc from to val released promises2_tgt)
-        (INV1: sem none_for inv promises1_src promises1_tgt)
+        (INV1: sem pview inv promises1_src promises1_tgt)
         (SIM1: sim_memory mem1_src mem1_tgt)
         (LE1_SRC: Memory.le promises1_src mem1_src)
         (LE1_TGT: Memory.le promises1_tgt mem1_tgt)
         (FINITE1_TGT: Memory.finite promises1_tgt):
-      <<INV2: sem (unset loc to none_for) (set loc to inv) promises1_src promises2_tgt>> /\
+      <<INV2: sem (unset loc to pview) (set loc to inv) promises1_src promises2_tgt>> /\
       <<INV2': mem loc to inv = false>>.
   Proof.
     hexploit Memory.remove_future; eauto. i. des.
@@ -380,7 +380,7 @@ Module SimPromises.
           guardH o. des. subst. unguardH o. des; congr.
         * revert COND1. rewrite unset_o. condtac; ss. congr.
       + i. revert MEM. rewrite unset_o. condtac; ss. guardH o. i.
-        exploit NONEFOR; eauto. i. des.
+        exploit PVIEW; eauto. i. des.
         erewrite Memory.remove_o; eauto. condtac; ss; eauto.
         des. subst. unguardH o. des; congr.
       + i. erewrite Memory.remove_o; eauto.
@@ -397,11 +397,11 @@ Module SimPromises.
   Qed.
 
   Lemma remove_src
-        none_for inv
+        pview inv
         loc from to val released
         promises1_src mem1_src
         promises1_tgt mem1_tgt
-        (INV1: sem none_for inv promises1_src promises1_tgt)
+        (INV1: sem pview inv promises1_src promises1_tgt)
         (INV1': mem loc to inv)
         (SIM1: sim_memory mem1_src mem1_tgt)
         (GET: Memory.get loc to promises1_src = Some (from, Message.mk val released))
@@ -409,7 +409,7 @@ Module SimPromises.
         (LE1_TGT: Memory.le promises1_tgt mem1_tgt):
     exists promises2_src,
       <<REMOVE_SRC: Memory.remove promises1_src loc from to val released promises2_src>> /\
-      <<INV2: sem none_for (unset loc to inv) promises2_src promises1_tgt>>.
+      <<INV2: sem pview (unset loc to inv) promises2_src promises1_tgt>>.
   Proof.
     inv INV1.
     exploit Memory.remove_exists; eauto. i. des.
@@ -418,7 +418,7 @@ Module SimPromises.
     - ii. revert LHS.
       erewrite (@Memory.remove_o mem2); eauto. condtac; ss; eauto.
       des. subst. exploit SOUND; eauto. i. des. congr.
-    - i. exploit NONEFOR; eauto.
+    - i. exploit PVIEW; eauto.
     - i. rewrite unset_o in INV. revert INV. condtac; ss.
       guardH o.
       i. exploit SOUND; eauto. i. des. splits; eauto.
@@ -431,21 +431,21 @@ Module SimPromises.
   Qed.
 
   Lemma remove
-        none_for inv
+        pview inv
         loc from to val released
         promises1_src mem1_src
         promises1_tgt mem1_tgt promises2_tgt
         (REL_WF: View.opt_wf released)
         (TIME: Time.lt from to)
         (REMOVE_TGT: Memory.remove promises1_tgt loc from to val released promises2_tgt)
-        (INV1: sem none_for inv promises1_src promises1_tgt)
+        (INV1: sem pview inv promises1_src promises1_tgt)
         (SIM1: sim_memory mem1_src mem1_tgt)
         (LE1_SRC: Memory.le promises1_src mem1_src)
         (LE1_TGT: Memory.le promises1_tgt mem1_tgt)
         (FINITE1_TGT: Memory.finite promises1_tgt):
     exists promises2_src,
-      <<REMOVE_SRC: Memory.remove promises1_src loc from to val (none_if loc to none_for released) promises2_src>> /\
-      <<INV2: sem (unset loc to none_for) inv promises2_src promises2_tgt>>.
+      <<REMOVE_SRC: Memory.remove promises1_src loc from to val (none_if loc to pview released) promises2_src>> /\
+      <<INV2: sem (unset loc to pview) inv promises2_src promises2_tgt>>.
   Proof.
     hexploit Memory.remove_future; try apply REMOVE_TGT; eauto. i. des.
     exploit remove_tgt; eauto. i. des.
@@ -481,11 +481,11 @@ Module SimPromises.
   Qed.
 
   Lemma future_aux_imm
-        none_for inv
+        pview inv
         promises_src mem1_src mem2_src
         promises_tgt mem1_tgt
         (FUTURE_SRC: Memory.future_imm mem1_src mem2_src)
-        (INV1: sem none_for inv promises_src promises_tgt)
+        (INV1: sem pview inv promises_src promises_tgt)
         (SIM1: sim_memory mem1_src mem1_tgt)
         (LE1_SRC: Memory.le promises_src mem1_src)
         (LE1_TGT: Memory.le promises_tgt mem1_tgt)
@@ -521,11 +521,11 @@ Module SimPromises.
   Qed.
 
   Lemma future_aux
-        none_for inv
+        pview inv
         promises_src mem1_src mem2_src
         promises_tgt mem1_tgt
         (FUTURE_SRC: Memory.future mem1_src mem2_src)
-        (INV1: sem none_for inv promises_src promises_tgt)
+        (INV1: sem pview inv promises_src promises_tgt)
         (SIM1: sim_memory mem1_src mem1_tgt)
         (LE1_SRC: Memory.le promises_src mem1_src)
         (LE1_TGT: Memory.le promises_tgt mem1_tgt)
@@ -564,10 +564,10 @@ Module SimPromises.
   Qed.
 
   Lemma future
-        none_for inv
+        pview inv
         lc_src mem1_src mem2_src
         lc_tgt mem1_tgt
-        (INV1: sem none_for inv lc_src.(Local.promises) lc_tgt.(Local.promises))
+        (INV1: sem pview inv lc_src.(Local.promises) lc_tgt.(Local.promises))
         (MEM1: sim_memory mem1_src mem1_tgt)
         (FUTURE_SRC: Memory.future mem1_src mem2_src)
         (WF1_SRC: Local.wf lc_src mem1_src)
