src/lang/MemoryFacts.v
@@ -171,16 +171,24 @@ Module MemoryFacts.
     - inv MEM. inv LOWER. inv TS0.
   Qed.
 
+  Lemma add_remove_eq
+        mem1 mem2 mem3 loc from from' to val val' rel rel'
+        (ADD: Memory.add mem1 loc from to val rel mem2)
+        (REMOVE: Memory.remove mem2 loc from' to val' rel' mem3):
+    mem3 = mem1.
+  Proof.
+    apply Memory.ext. i.
+    erewrite (@Memory.remove_o mem3); eauto.
+    erewrite (@Memory.add_o mem2); eauto.
+    condtac; ss. des. subst. symmetry. eauto using Memory.add_get0.
+  Qed.
+
   Lemma write_add_promises
         promises1 mem1 loc from to val released promises2 mem2
         (WRITE: Memory.write promises1 mem1 loc from to val released promises2 mem2 Memory.op_kind_add):
     promises2 = promises1.
   Proof.
-    apply Memory.ext. i.
-    inv WRITE. inv PROMISE.
-    erewrite (@Memory.remove_o promises2); eauto. condtac; ss.
-    - des. subst. symmetry. eapply Memory.add_get0. eauto.
-    - guardH o. erewrite (@Memory.add_o promises0); eauto. condtac; ss.
+    inv WRITE. inv PROMISE. eapply add_remove_eq; eauto.
   Qed.
 
   Lemma promise_exists_None
@@ -197,13 +205,14 @@ Module MemoryFacts.
     esplits. econs; eauto. apply Time.bot_spec.
   Qed.
 
-  Lemma some_released_time_lt
-  mem loc from to val released
-  (CLOSED: Memory.closed mem)
-  (GET: Memory.get loc to mem = Some (from, Message.mk val (Some released))):
+  Lemma released_time_lt
+        mem loc from to val released
+        (CLOSED: Memory.closed mem)
+        (GET: Memory.get loc to mem = Some (from, Message.mk val (Some released))):
     Time.lt from to.
   Proof.
     destruct (mem loc).(Cell.WF). exploit VOLUME; eauto. i. des; ss. inv x.
     inv CLOSED. rewrite INHABITED in GET. inv GET.
   Qed.
+
 End MemoryFacts.
